ulib/LowStar.Permissions.Array.fsti
@@ -1,0 +1,87 @@
+module LowStar.Permissions.Array
+
+module HS = FStar.HyperStack
+open FStar.HyperStack.ST
+module U32 = FStar.UInt32
+
+val array (a:Type0): Type0
+
+(*** Definitions of Ghost operations and predicates on arrays ***)
+
+val length (#a:Type) (b:array a) : nat
+
+val live (#a:Type) (h:HS.mem) (b:array a) : Type0
+val writeable (#a:Type) (h:HS.mem) (b:array a) : Type0
+
+val lemma_writeable_implies_live (#a:Type) (h:HS.mem) (b:array a)
+  : Lemma (requires writeable h b)
+          (ensures live h b)
+
+val as_seq (#a:Type) (h:HS.mem) (b:array a) : GTot (s:Seq.seq a{Seq.length s == length b})
+
+let get (#a:Type) (h:HS.mem) (b:array a) (i:nat{i < length b}) : GTot a
+  = Seq.index (as_seq h b) i
+
+val mergeable (#a:Type0) (b1 b2:array a) : Type0
+
+val frameOf (#a:Type0) (b:array a) : Tot HS.rid
+val as_addr (#a:Type0) (b:array a) : GTot nat
+
+(*** Definitions of locations for arrays with permissions ***)
+
+val bloc:Type0
+
+val loc_none: bloc
+val loc_union (s1 s2: bloc) : GTot bloc
+val loc_disjoint (s1 s2: bloc) : GTot Type0
+val loc_includes (s1 s2: bloc) : GTot Type0
+
+val loc_array (#a:Type0) (b:array a) : GTot bloc
+
+val modifies (s: bloc) (h1 h2: HS.mem) : GTot Type0
+
+(*** Stateful operations implementing the ghost specifications ***)
+
+
+val index (#a:Type) (b:array a) (i:U32.t{U32.v i < length b})
+  : Stack a (requires fun h -> live h b)
+            (ensures fun h0 y h1 -> h0 == h1 /\ y == get h0 b (U32.v i))
+
+val upd (#a:Type) (b:array a) (i:U32.t{U32.v i < length b}) (v:a)
+    : Stack unit (requires fun h -> writeable h b)
+                 (ensures fun h0 _ h1 ->  writeable h1 b /\
+                                       modifies (loc_array b) h0 h1 /\
+                                       as_seq h1 b == Seq.upd (as_seq h0 b) (U32.v i) v)
+
+
+// TODO: Do we want split instead
+val gsub (#a:Type0) (b:array a) (i:U32.t) (len:U32.t)
+  :Ghost (array a)
+         (requires (U32.v i + U32.v len <= length b))
+	 (ensures (fun _ -> True))
+
+
+val sub (#a:Type) (b:array a) (i:U32.t) (len:U32.t)
+  : Stack (array a)
+          (requires fun h -> U32.v i + U32.v len <= length b /\ live h b)
+          (ensures fun h0 y h1 -> h0 == h1 /\ y == gsub b i len)
+
+
+val alloc (#a:Type0) (init:a) (len:U32.t)
+  : ST (array a)
+       (requires fun _ -> U32.v len > 0)
+       (ensures fun h0 b h1 -> 
+         modifies loc_none h0 h1 /\ 
+         writeable h1 b /\ 
+         as_seq h1 b == Seq.create (U32.v len) init)
+
+val share (#a:Type0) (b:array a) : Stack (array a)
+  (requires fun h0 -> live h0 b /\ length b > 0)
+  (ensures fun h0 b' h1 -> 
+    modifies (loc_array b) h0 h1 /\ 
+    live h1 b /\ live h1 b' /\
+    loc_disjoint (loc_array b) (loc_array b') /\
+    as_seq h0 b == as_seq h1 b /\ // The values of the initial array are not modified
+    as_seq h1 b' == as_seq h1 b /\ // The values of the new buffer are the same as the initial array
+    mergeable b b' /\
+    True) // TODO: Talk about permissions here?
